first CESK; will refactor

AAM.v
@@ -2,6 +2,8 @@
 
 Require Export SfLib.
 
+(* ###################################################################### *)
+
 Inductive expr : Type :=
   | var : id -> expr
   | app : expr -> expr -> expr
@@ -11,18 +13,20 @@ Tactic Notation "expr_cases" tactic(first) ident(c) :=
   first;
   [ Case_aux c "var" | Case_aux c "app" | Case_aux c "abs" ].
 
+(* ###################################################################### *)
+
 Module CEK.
 
 Inductive val : Type :=
   | clo : id -> expr -> partial_map val -> val.
 
-Definition env := partial_map val.
+Definition env : Type := partial_map val.
 
 Inductive frame : Type :=
   | ar : expr -> frame
   | fn : val -> frame.
 
-Definition kont := list frame.
+Definition kont : Type := list frame.
 
 Inductive state : Type :=
   | ev : expr -> env -> kont -> state
@@ -70,11 +74,13 @@ Tactic Notation "step_cases" tactic(first) ident(c) :=
 
 Hint Constructors step.
 
-Notation "t1 '==>*' t2" := (multi step t1 t2) (at level 40).
+Notation "s1 '==>*' s2" := (multi step s1 s2) (at level 40).
 
 Example ex1 :
   forall x y,
-    inj (app (abs x (var x)) (abs y (var y))) ==>* ap (clo y (var y) empty) [].
+    inj (app (abs x (var x)) (abs y (var y)))
+    ==>*
+    ap (clo y (var y) empty) [].
 Proof.
   intros. unfold inj.
   eapply multi_step. auto.
@@ -88,3 +94,92 @@ Qed.
 
 End CEK.
 
+(* ###################################################################### *)
+
+Module CESK.
+
+Definition addr : Type := id.
+       
+Inductive val : Type :=
+  | clo : id -> expr -> partial_map addr -> val.
+
+Definition env : Type := partial_map addr.
+
+Definition storable : Type := val.
+
+Definition store : Type := partial_map storable.
+
+Inductive frame : Type :=
+  | ar : expr -> frame
+  | fn : val -> frame.
+
+Definition kont : Type := list frame.
+
+Inductive state : Type :=
+  | ev : expr -> env -> store -> kont -> state
+  | ap : val -> store -> kont -> state.
+
+Definition inj : expr -> state :=
+  fun e => ev e empty empty [].
+
+Reserved Notation "s1 '==>' s2" (at level 40).
+
+Inductive step : state -> state -> Prop :=
+  | cesk1 :
+      forall x p s k a v,
+        p x = Some a ->
+        s a = Some v ->
+        ev (var x) p s k
+        ==>
+        ap v s k
+  | cesk2 :
+      forall x e p s k,
+        ev (abs x e) p s k
+        ==>
+        ap (clo x e p) s k
+  | cesk3 :
+      forall e1 e2 p s k,
+        ev (app e1 e2) p s k
+        ==>
+        ev e1 p s (ar e2 :: k)
+  | cesk4 :
+      forall x e p s e2 k,
+        ap (clo x e p) s (ar e2 :: k)
+        ==>
+        ev e2 p s (fn (clo x e p) :: k)
+  | cesk5 :
+      forall x e p s v2 k a,
+        s a = None ->
+        ap v2 s (fn (clo x e p) :: k)
+        ==>
+        ev e (extend p x a) (extend s a v2) k
+
+where "s1 '==>' s2" := (step s1 s2).
+
+Tactic Notation "step_cases" tactic(first) ident(c) :=
+  first;
+  [ Case_aux c "cesk1" | Case_aux c "cesk2" | Case_aux c "cesk3"
+    | Case_aux c "cesk4" | Case_aux c "cesk5" ].
+
+Hint Constructors step.
+
+Notation "s1 '==>*' s2" := (multi step s1 s2) (at level 40).
+
+Example ex1 :
+  forall x y,
+    inj (app (abs x (var x)) (abs y (var y)))
+    ==>*
+    ap (clo y (var y) empty) (extend empty (Id 0) (clo y (var y) empty)) [].
+Proof.
+  intros. unfold inj.
+  eapply multi_step. auto.
+  eapply multi_step. auto.
+  eapply multi_step. auto.
+  eapply multi_step. auto.
+  eapply multi_step. apply cesk5. auto.
+  eapply multi_step. apply cesk1 with (Id 0). apply extend_eq.
+    unfold extend. simpl. auto.
+  apply multi_refl.
+Qed.
+
+End CESK.
